src/crypto/aes/ctr.s.dfy
@@ -43,53 +43,56 @@ function CTR_Encrypt_At(inp : Quadword, key : seq<uint32>, alg: Algorithm, iv : 
 
 function CTR_Encrypt'(inp : seq<Quadword>, key : seq<uint32>, alg: Algorithm, iv : uint64, init_ctr : uint64, n : uint64) : seq<Quadword>
     requires CTR_Encrypt_Req(inp, key, alg);
-    requires |inp| + n < 0x1_0000_0000_0000_0000 - 1;
+    requires |inp| < 0x1_0000_0000_0000_0000 - 1;
     decreases |inp|;
 {
    if |inp| == 1 then
     [CTR_Encrypt_At(inp[0], key, alg, iv, init_ctr, n)]
     else
       [CTR_Encrypt_At(inp[0], key, alg, iv, init_ctr, n)] +
-       CTR_Encrypt'(inp[1..], key, alg, iv, init_ctr, n + 1)
+       CTR_Encrypt'(inp[1..], key, alg, iv, init_ctr, BitwiseAdd64(n,1))
 }
 
 lemma lemma_CTR_Encrypt_length_specific(inp : seq<Quadword>, key:seq<uint32>, alg:Algorithm, iv: uint64, init_ctr : uint64, n : uint64) 
     requires CTR_Encrypt_Req(inp, key, alg);
-    requires 0 < |inp| + n < 0x1_0000_0000_0000_0000 - 1
+    requires 0 < |inp| < 0x1_0000_0000_0000_0000 - 1
     decreases |inp|;
     ensures  |CTR_Encrypt'(inp, key, alg, iv, init_ctr, n)| == |inp|;
 {
     if |inp| == 1 {
       assert |CTR_Encrypt'(inp, key, alg, iv, init_ctr, n)| == 1;
     } else {
-        lemma_CTR_Encrypt_length_specific(inp[1..], key, alg, iv, init_ctr, n);
+      lemma_CTR_Encrypt_length_specific(inp[1..], key, alg, iv, init_ctr, BitwiseAdd64(n,1));
     }
 }
-
-/*
-
-lemma lemma_CTR_Encrypt_length(inp : seq<Quadword>, key:seq<uint32>, alg:Algorithm, iv: uint64, init_ctr : uint64) 
-    requires CTR_Encrypt_Req(inp, key, alg);
-    requires 0 < |inp| < 0x1_0000_0000_0000_0000 - 1
-    ensures forall inp :: |inp| > 0 ==> |CTR_Encrypt'(inp, key, alg, iv, init_ctr,0)| == |inp|;
-    decreases |inp|;
-{
-    forall inp | |inp| > 0
-        ensures |CTR_Encrypt'(inp, key, alg, iv, init_ctr,0)| == |inp|;
-    {
-        lemma_CTR_Encrypt_length_specific(inp, key, alg, iv, init_ctr);
-    }
-}
-
 
 function CTR_Encrypt(inp : seq<Quadword>, key : seq<uint32>, alg: Algorithm, iv : uint64, init_ctr : uint64) : seq<Quadword>
   requires CTR_Encrypt_Req(inp, key, alg);
   ensures  |CTR_Encrypt(inp, key, alg, iv, init_ctr)| == |inp|;
 {
-//   lemma_CTR_Encrypt_length(inp, key, alg, iv, init_ctr);
+   lemma_CTR_Encrypt_length_specific(inp, key, alg, iv, init_ctr, 0);
    CTR_Encrypt'(inp, key, alg, iv, init_ctr, 0)
 }
 
-*/
+// An unused alternative specification, as recursive functions are closer to the original spec.
+
+predicate CTR_Encrypt_Is(inp : seq<Quadword>, key : seq<uint32>, alg: Algorithm, iv : uint64, init_ctr : uint64, outp : seq<Quadword>) 
+    requires CTR_Encrypt_Req(inp, key, alg);
+{
+ |inp| == |outp| &&
+  forall i : nat :: 0 <= i < |inp| ==>
+    outp[i] == CTR_Encrypt_At(inp[i], key, alg, iv, init_ctr, i)
+}
+
+
+predicate CTR_Encrypt_Upto(inp : seq<Quadword>, key : seq<uint32>, alg: Algorithm, iv : uint64, init_ctr : uint64, outp : seq<Quadword>, upto : nat) 
+    requires upto < |inp|;
+    requires CTR_Encrypt_Req(inp, key, alg);
+{
+ |inp| == |outp| &&
+  forall i : nat :: 0 <= i < upto ==>
+    outp[i] == CTR_Encrypt_At(inp[i], key, alg, iv, init_ctr, i)
+}
+
 // We don't need a decrypt predicate as the standard uses encrypt again and the xor decrypts.
 }
