src/crypto/aes/aes-x64/proof.dfy
@@ -1,0 +1,100 @@
+include "../../../lib/util/types.s.dfy"
+include "../../../lib/util/operations.s.dfy"
+include "../../../lib/util/words_and_bytes.s.dfy"
+include "../../../lib/collections/Seqs.s.dfy"
+include "../../../arch/x64/vale.i.dfy"
+include "../../../arch/x64/vale64.i.dfy"
+include "../../../lib/util/dafny_wrappers.i.dfy"
+include "../ctr.s.dfy"
+include "../aes.s.dfy"
+//include "../aes_helpers.i.dfy"
+include "ctr_helpers.i.dfy"
+
+module proof {
+
+import opened x64_vale_i
+import opened x64_def_s
+import opened types_s
+import opened dafny_wrappers_i
+import opened AESModule
+//import opened AESHelpersModule
+import opened CTRModule
+import opened CTRHelpers
+
+/*
+lemma lemma_BitwiseAdd64xy(x : uint64, y: uint64)
+    ensures  x + y < 0x1_0000_0000_0000_0000 ==> BitwiseAdd64(x, y) == x + y
+    ensures  x + y >= 0x1_0000_0000_0000_0000 ==> BitwiseAdd64(x, y) == x + y - 0x1_0000_0000_0000_0000
+    ensures  forall x:uint64 :: BitwiseAdd64(x, 0) == x;
+{
+    reveal_BitwiseAdd64();
+}
+
+lemma {:timeLimitMultiplier 6} lemma_CTR_Encrypt'_Is(inp : seq<Quadword>, key : seq<uint32>, alg : Algorithm, iv : uint64, init_ctr : uint64, n : uint64, i : nat)
+  requires CTR_Encrypt_Req(inp, key, alg);
+  requires 0 < |inp| < 0x1_0000_0000_0000_0000 - 1;
+  requires i < |inp|;
+  ensures |CTR_Encrypt'(inp, key, alg, iv, init_ctr, n)| == |inp|;
+  ensures 
+    CTR_Encrypt'(inp, key, alg, iv, init_ctr, n)[i] == 
+      QuadwordXor(inp[i], AES_Encrypt(key, ctr_n(iv, init_ctr, BitwiseAdd64(n,i)), alg));
+{
+  lemma_CTR_Encrypt'_length(inp);
+  lemma_BitwiseAdd64xy(n,1); // works but times out a lot.
+  if i == 0 {
+    assert
+      CTR_Encrypt'(inp, key, alg, iv, init_ctr, n)[0] == 
+       QuadwordXor(inp[0], AES_Encrypt(key, ctr_n(iv, init_ctr, n), alg));
+  } else {
+    lemma_CTR_Encrypt'_Is(inp[1..], key, alg, iv, init_ctr, BitwiseAdd64(n,1), i - 1);
+  }
+}
+*/
+
+
+lemma{:timeLimitMultiplier 6} lemma_CTR_Encrypt'_Is(inp : seq<Quadword>, key : seq<uint32>, alg : Algorithm, iv : uint64, init_ctr : uint64, n : uint64) 
+  requires CTR_Encrypt_Req(inp, key, alg);
+  requires 0 < |inp| < 0x1_0000_0000_0000_0000 - 1;
+  ensures |CTR_Encrypt'(inp, key, alg, iv, init_ctr, n)| == |inp|;
+  ensures forall i : nat :: i < |inp| ==>
+   CTR_Encrypt'(inp, key, alg, iv, init_ctr, n)[i] == 
+    QuadwordXor(inp[i], AES_Encrypt(key, ctr_n(iv, init_ctr, BitwiseAdd64(n,i)), alg));
+{
+  lemma_CTR_Encrypt'_length(inp);
+  lemma_BitwiseAdd64(); // works but times out a lot.
+  //lemma_BitwiseAdd64xy(n,i);
+  //lemma_BitwiseAdd64xy(n,1);
+  if |inp| == 1 {
+    assert
+      CTR_Encrypt'(inp, key, alg, iv, init_ctr, n)[0] == 
+       QuadwordXor(inp[0], AES_Encrypt(key, ctr_n(iv, init_ctr, n), alg));
+  } else {
+    lemma_CTR_Encrypt'_Is(inp[1..], key, alg, iv, init_ctr, BitwiseAdd64(n,1));
+  }
+}
+
+/*
+
+lemma{:timeLimitMultiplier 6} lemma_CTR_Encrypt_Is'(inp : seq<Quadword>, key : seq<uint32>, alg : Algorithm, iv : uint64, init_ctr : uint64) 
+  requires CTR_Encrypt_Req(inp, key, alg);
+  requires 0 < |inp| < 0x1_0000_0000_0000_0000 - 1;
+  ensures |CTR_Encrypt(inp, key, alg, iv, init_ctr)| == |inp|;
+  ensures CTR_Encrypt(inp, key, alg, iv, init_ctr) == CTR_Encrypt'(inp, key, alg, iv, init_ctr, 0);
+{
+  lemma_CTR_Encrypt_length(inp);
+}
+
+
+lemma{:timeLimitMultiplier 3} lemma_CTR_Encrypt_Is(inp : seq<Quadword>, key : seq<uint32>, alg : Algorithm, iv : uint64, init_ctr : uint64) 
+  requires CTR_Encrypt_Req(inp, key, alg);
+  requires 0 < |inp| < 0x1_0000_0000_0000_0000 - 1;
+  ensures |CTR_Encrypt(inp, key, alg, iv, init_ctr)| == |inp|;
+  ensures forall i : nat :: i < |inp| ==> 
+    CTR_Encrypt(inp, key, alg, iv, init_ctr)[i] == CTR_Encrypt'(inp, key, alg, iv, init_ctr, 0)[i];
+{
+  lemma_CTR_Encrypt_length(inp);
+  lemma_CTR_Encrypt_Is'(inp, key, alg, iv, init_ctr);
+}
+*/
+
+}
